copy-parse bytes

src/cddl/pulse/CDDL.Pulse.Parse.Misc.fst
@@ -85,3 +85,78 @@ let impl_copyful_int_range_neg_int64
     (lo hi: Ghost.erased U64.t)
 : impl_copyful_parse vmatch (spec_int_range_neg_int64 lo hi).parser (rel_pure U64.t)
 = impl_copyful_ext (impl_copyful_nint cbor_destr_int64) (spec_int_range_neg_int64 lo hi).parser ()
+
+module U8 = FStar.UInt8
+module SZ = FStar.SizeT
+module S = Pulse.Lib.Slice
+module V = Pulse.Lib.Vec
+module A = Pulse.Lib.Array
+
+inline_for_extraction noextract [@@noextract_to "krml"]
+```pulse
+fn impl_copyful_bytes_gen
+    (#ty: Type u#0)
+    (#vmatch: perm -> ty -> cbor -> slprop)
+    (cbor_destr_string: get_string_t vmatch)
+    (#t: Ghost.erased typ)
+    (#ser: Ghost.erased (Seq.seq U8.t -> bool))
+    (par: Ghost.erased (parser_spec t (Seq.seq U8.t) ser))
+    (sq: squash (
+      forall (x: cbor) . Ghost.reveal t x ==> (CString? (unpack x) /\ (Ghost.reveal par x <: Seq.seq U8.t) == CString?.v (unpack x))
+    ))
+: impl_copyful_parse #ty vmatch #(Ghost.reveal t) #(Seq.seq U8.t) #(Ghost.reveal ser) (Ghost.reveal par) #_ (rel_vec_or_slice_of_seq true)
+=
+    (c: ty)
+    (#p: perm)
+    (#v: Ghost.erased cbor)
+{
+  let s = cbor_destr_string c;
+  with ps vs . assert (pts_to s #ps vs);
+  let len = S.len s;
+  S.pts_to_len s;
+  let len64 = SZ.sizet_to_uint64 len;
+  let v = V.alloc 0uy len;
+  V.to_array_pts_to v;
+  let s' = S.from_array (V.vec_to_array v) len;
+  S.pts_to_len s';
+  S.copy s' s;
+  Trade.elim _ _; // release s
+  S.to_array s';
+  V.to_vec_pts_to v;
+  let w : vec U8.t = {
+    len = len64;
+    v = v;
+  };
+  rewrite (pts_to v vs) as (pts_to w.v vs);
+  fold (rel_vec_of_seq w vs);
+  let res : vec_or_slice U8.t = Vec w;
+  fold (rel_vec_or_slice_of_seq true res vs);
+  res
+}
+```
+
+inline_for_extraction noextract [@@noextract_to "krml"]
+let impl_copyful_bytes
+    (#ty: Type u#0)
+    (#vmatch: perm -> ty -> cbor -> slprop)
+    (cbor_destr_string: get_string_t vmatch)
+: impl_copyful_parse #ty vmatch #bstr #(Seq.seq U8.t) #_ spec_bstr.parser #_ (rel_vec_or_slice_of_seq true )
+= impl_copyful_bytes_gen cbor_destr_string _ ()
+
+inline_for_extraction noextract [@@noextract_to "krml"]
+let impl_copyful_text
+    (#ty: Type u#0)
+    (#vmatch: perm -> ty -> cbor -> slprop)
+    (cbor_destr_string: get_string_t vmatch)
+: impl_copyful_parse #ty vmatch #tstr #(Seq.seq U8.t) #_ spec_tstr.parser #_ (rel_vec_or_slice_of_seq true )
+= impl_copyful_bytes_gen cbor_destr_string _ ()
+
+inline_for_extraction noextract [@@noextract_to "krml"]
+let impl_copyful_str_size
+    (#ty: Type u#0)
+    (#vmatch: perm -> ty -> cbor -> slprop)
+    (cbor_destr_string: get_string_t vmatch)
+    (mt: Ghost.erased major_type_byte_string_or_text_string)
+    (lo hi: Ghost.erased U64.t)
+: impl_copyful_parse vmatch (spec_str_size mt lo hi).parser (rel_vec_or_slice_of_seq true)
+= impl_copyful_bytes_gen cbor_destr_string _ ()
